coqimp/contextswitch/lib/integer_lemma.v
@@ -1,0 +1,1107 @@
+Require Import Coqlib.                         
+Require Import Maps.           
+Require Import LibTactics.   
+        
+Require Import Integers.  
+Open Scope Z_scope.        
+Import ListNotations.  
+   
+Set Asymmetric Patterns.  
+        
+Require Import state.    
+Require Import language. 
+ 
+Set Implicit Arguments.    
+Unset Strict Implicit. 
+
+Require Import Coq.Logic.FunctionalExtensionality.
+
+Open Scope nat.
+Open Scope code_scope.
+Open Scope mem_scope.
+
+(*+ Lemmas about Integers +*)
+Lemma in_range0 :
+  ($ (-4096)) <=ᵢ ($ 0) && ($ 0) <=ᵢ ($ 4095) = true.
+Proof.
+  unfold orb.
+  unfold Int.lt.
+  unfold Int.eq.
+  destruct (zlt (Int.signed $ (-4096)) (Int.signed $ 0)) eqn:Heqe;
+    destruct (zeq (Int.unsigned $ (-4096)) (Int.unsigned $ 0)) eqn:Heqe1;
+    destruct (zlt (Int.signed $ 0) (Int.signed $ 4095)) eqn:Heqe2;
+    destruct (zeq (Int.unsigned $ 0) (Int.unsigned $ 4095)) eqn:Heqe3; eauto; tryfalse.
+Qed.
+
+Lemma in_range1 :
+  ($ (-4096)) <=ᵢ ($ 1) && ($ 1) <=ᵢ ($ 4095) = true.
+Proof.
+  unfold orb.
+  unfold Int.lt.
+  unfold Int.eq.
+  destruct (zlt (Int.signed $ (-4096)) (Int.signed $ 1)) eqn:Heqe;
+    destruct (zeq (Int.unsigned $ (-4096)) (Int.unsigned $ 1)) eqn:Heqe1;
+    destruct (zlt (Int.signed $ 1) (Int.signed $ 4095)) eqn:Heqe2;
+    destruct (zeq (Int.unsigned $ 1) (Int.unsigned $ 4095)) eqn:Heqe3; eauto; tryfalse.
+Qed.
+
+Lemma in_range4 :
+  ($ (-4096)) <=ᵢ ($ 4) && ($ 4) <=ᵢ ($ 4095) = true.
+Proof.
+  unfold orb.
+  unfold Int.lt.
+  unfold Int.eq.
+  destruct (zlt (Int.signed $ (-4096)) (Int.signed $ 4)) eqn:Heqe;
+    destruct (zeq (Int.unsigned $ (-4096)) (Int.unsigned $ 4)) eqn:Heqe1;
+    destruct (zlt (Int.signed $ 4) (Int.signed $ 4095)) eqn:Heqe2;
+    destruct (zeq (Int.unsigned $ 4) (Int.unsigned $ 4095)) eqn:Heqe3; eauto; tryfalse.
+Qed.
+
+Lemma in_range7 :
+  ($ (-4096)) <=ᵢ ($ 7) && ($ 7) <=ᵢ ($ 4095) = true.
+Proof.
+  unfold orb.
+  unfold Int.lt.
+  unfold Int.eq.
+  destruct (zlt (Int.signed $ (-4096)) (Int.signed $ 7)) eqn:Heqe;
+    destruct (zeq (Int.unsigned $ (-4096)) (Int.unsigned $ 7)) eqn:Heqe1;
+    destruct (zlt (Int.signed $ 7) (Int.signed $ 4095)) eqn:Heqe2;
+    destruct (zeq (Int.unsigned $ 7) (Int.unsigned $ 4095)) eqn:Heqe3; eauto; tryfalse.
+Qed.
+
+Lemma in_range8 :
+  ($ (-4096)) <=ᵢ ($ 8) && ($ 8) <=ᵢ ($ 4095) = true.
+Proof.
+  unfold orb.
+  unfold Int.lt.
+  unfold Int.eq.
+  destruct (zlt (Int.signed $ (-4096)) (Int.signed $ 8)) eqn:Heqe;
+    destruct (zeq (Int.unsigned $ (-4096)) (Int.unsigned $ 8)) eqn:Heqe1;
+    destruct (zlt (Int.signed $ 8) (Int.signed $ 4095)) eqn:Heqe2;
+    destruct (zeq (Int.unsigned $ 8) (Int.unsigned $ 4095)) eqn:Heqe3; eauto; tryfalse.
+Qed.
+
+Lemma in_range12 :
+  ($ (-4096)) <=ᵢ ($ 12) && ($ 12) <=ᵢ ($ 4095) = true.
+Proof.
+  unfold orb.
+  unfold Int.lt.
+  unfold Int.eq.
+  destruct (zlt (Int.signed $ (-4096)) (Int.signed $ 12)) eqn:Heqe;
+    destruct (zeq (Int.unsigned $ (-4096)) (Int.unsigned $ 12)) eqn:Heqe1;
+    destruct (zlt (Int.signed $ 12) (Int.signed $ 4095)) eqn:Heqe2;
+    destruct (zeq (Int.unsigned $ 12) (Int.unsigned $ 4095)) eqn:Heqe3; eauto; tryfalse.
+Qed.
+
+Lemma in_range16 :
+  ($ (-4096)) <=ᵢ ($ 16) && ($ 16) <=ᵢ ($ 4095) = true.
+Proof.
+  unfold orb.
+  unfold Int.lt.
+  unfold Int.eq.
+  destruct (zlt (Int.signed $ (-4096)) (Int.signed $ 12)) eqn:Heqe;
+    destruct (zeq (Int.unsigned $ (-4096)) (Int.unsigned $ 12)) eqn:Heqe1;
+    destruct (zlt (Int.signed $ 12) (Int.signed $ 4095)) eqn:Heqe2;
+    destruct (zeq (Int.unsigned $ 12) (Int.unsigned $ 4095)) eqn:Heqe3; eauto; tryfalse.
+Qed.
+
+Lemma in_range20 :
+  ($ (-4096)) <=ᵢ ($ 20) && ($ 20) <=ᵢ ($ 4095) = true.
+Proof.
+  unfold orb.
+  unfold Int.lt.
+  unfold Int.eq.
+  destruct (zlt (Int.signed $ (-4096)) (Int.signed $ 20)) eqn:Heqe;
+    destruct (zeq (Int.unsigned $ (-4096)) (Int.unsigned $ 20)) eqn:Heqe1;
+    destruct (zlt (Int.signed $ 20) (Int.signed $ 4095)) eqn:Heqe2;
+    destruct (zeq (Int.unsigned $ 20) (Int.unsigned $ 4095)) eqn:Heqe3; eauto; tryfalse.
+Qed.
+
+Lemma in_range24 :
+  ($ (-4096)) <=ᵢ ($ 24) && ($ 24) <=ᵢ ($ 4095) = true.
+Proof.
+  unfold orb.
+  unfold Int.lt.
+  unfold Int.eq.
+  destruct (zlt (Int.signed $ (-4096)) (Int.signed $ 24)) eqn:Heqe;
+    destruct (zeq (Int.unsigned $ (-4096)) (Int.unsigned $ 24)) eqn:Heqe1;
+    destruct (zlt (Int.signed $ 24) (Int.signed $ 4095)) eqn:Heqe2;
+    destruct (zeq (Int.unsigned $ 24) (Int.unsigned $ 4095)) eqn:Heqe3; eauto; tryfalse.
+Qed.
+
+Lemma in_range28 :
+  ($ (-4096)) <=ᵢ ($ 28) && ($ 28) <=ᵢ ($ 4095) = true.
+Proof.
+  unfold orb.
+  unfold Int.lt.
+  unfold Int.eq.
+  destruct (zlt (Int.signed $ (-4096)) (Int.signed $ 28)) eqn:Heqe;
+    destruct (zeq (Int.unsigned $ (-4096)) (Int.unsigned $ 28)) eqn:Heqe1;
+    destruct (zlt (Int.signed $ 28) (Int.signed $ 4095)) eqn:Heqe2;
+    destruct (zeq (Int.unsigned $ 28) (Int.unsigned $ 4095)) eqn:Heqe3; eauto; tryfalse.
+Qed.
+
+Lemma in_range32 :
+  ($ (-4096)) <=ᵢ ($ 32) && ($ 32) <=ᵢ ($ 4095) = true.
+Proof.
+  unfold orb.
+  unfold Int.lt.
+  unfold Int.eq.
+  destruct (zlt (Int.signed $ (-4096)) (Int.signed $ 32)) eqn:Heqe;
+    destruct (zeq (Int.unsigned $ (-4096)) (Int.unsigned $ 32)) eqn:Heqe1;
+    destruct (zlt (Int.signed $ 32) (Int.signed $ 4095)) eqn:Heqe2;
+    destruct (zeq (Int.unsigned $ 32) (Int.unsigned $ 4095)) eqn:Heqe3; eauto; tryfalse.
+Qed.
+
+Lemma in_range36 :
+  ($ (-4096)) <=ᵢ ($ 36) && ($ 36) <=ᵢ ($ 4095) = true.
+Proof.
+  unfold orb.
+  unfold Int.lt.
+  unfold Int.eq.
+  destruct (zlt (Int.signed $ (-4096)) (Int.signed $ 36)) eqn:Heqe;
+    destruct (zeq (Int.unsigned $ (-4096)) (Int.unsigned $ 36)) eqn:Heqe1;
+    destruct (zlt (Int.signed $ 36) (Int.signed $ 4095)) eqn:Heqe2;
+    destruct (zeq (Int.unsigned $ 36) (Int.unsigned $ 4095)) eqn:Heqe3; eauto; tryfalse.
+Qed.
+
+Lemma in_range40 :
+  ($ (-4096)) <=ᵢ ($ 40) && ($ 40) <=ᵢ ($ 4095) = true.
+Proof.
+  unfold orb.
+  unfold Int.lt.
+  unfold Int.eq.
+  destruct (zlt (Int.signed $ (-4096)) (Int.signed $ 40)) eqn:Heqe;
+    destruct (zeq (Int.unsigned $ (-4096)) (Int.unsigned $ 40)) eqn:Heqe1;
+    destruct (zlt (Int.signed $ 40) (Int.signed $ 4095)) eqn:Heqe2;
+    destruct (zeq (Int.unsigned $ 40) (Int.unsigned $ 4095)) eqn:Heqe3; eauto; tryfalse.
+Qed.
+
+Lemma in_range44 :
+  ($ (-4096)) <=ᵢ ($ 44) && ($ 44) <=ᵢ ($ 4095) = true.
+Proof.
+  unfold orb.
+  unfold Int.lt.
+  unfold Int.eq.
+  destruct (zlt (Int.signed $ (-4096)) (Int.signed $ 44)) eqn:Heqe;
+    destruct (zeq (Int.unsigned $ (-4096)) (Int.unsigned $ 44)) eqn:Heqe1;
+    destruct (zlt (Int.signed $ 44) (Int.signed $ 4095)) eqn:Heqe2;
+    destruct (zeq (Int.unsigned $ 44) (Int.unsigned $ 4095)) eqn:Heqe3; eauto; tryfalse.
+Qed.
+
+Lemma in_range48 :
+  ($ (-4096)) <=ᵢ ($ 48) && ($ 48) <=ᵢ ($ 4095) = true.
+Proof.
+  unfold orb.
+  unfold Int.lt.
+  unfold Int.eq.
+  destruct (zlt (Int.signed $ (-4096)) (Int.signed $ 48)) eqn:Heqe;
+    destruct (zeq (Int.unsigned $ (-4096)) (Int.unsigned $ 48)) eqn:Heqe1;
+    destruct (zlt (Int.signed $ 48) (Int.signed $ 4095)) eqn:Heqe2;
+    destruct (zeq (Int.unsigned $ 48) (Int.unsigned $ 4095)) eqn:Heqe3; eauto; tryfalse.
+Qed.
+
+Lemma in_range52 :
+  ($ (-4096)) <=ᵢ ($ 52) && ($ 52) <=ᵢ ($ 4095) = true.
+Proof.
+  unfold orb.
+  unfold Int.lt.
+  unfold Int.eq.
+  destruct (zlt (Int.signed $ (-4096)) (Int.signed $ 52)) eqn:Heqe;
+    destruct (zeq (Int.unsigned $ (-4096)) (Int.unsigned $ 52)) eqn:Heqe1;
+    destruct (zlt (Int.signed $ 52) (Int.signed $ 4095)) eqn:Heqe2;
+    destruct (zeq (Int.unsigned $ 52) (Int.unsigned $ 4095)) eqn:Heqe3; eauto; tryfalse.
+Qed.
+
+Lemma in_range56 :
+  ($ (-4096)) <=ᵢ ($ 56) && ($ 56) <=ᵢ ($ 4095) = true.
+Proof.
+  unfold orb.
+  unfold Int.lt.
+  unfold Int.eq.
+  destruct (zlt (Int.signed $ (-4096)) (Int.signed $ 56)) eqn:Heqe;
+    destruct (zeq (Int.unsigned $ (-4096)) (Int.unsigned $ 56)) eqn:Heqe1;
+    destruct (zlt (Int.signed $ 56) (Int.signed $ 4095)) eqn:Heqe2;
+    destruct (zeq (Int.unsigned $ 56) (Int.unsigned $ 4095)) eqn:Heqe3; eauto; tryfalse.
+Qed.
+
+Lemma in_range60 :
+  ($ (-4096)) <=ᵢ ($ 60) && ($ 60) <=ᵢ ($ 4095) = true.
+Proof.
+  unfold orb.
+  unfold Int.lt.
+  unfold Int.eq.
+  destruct (zlt (Int.signed $ (-4096)) (Int.signed $ 60)) eqn:Heqe;
+    destruct (zeq (Int.unsigned $ (-4096)) (Int.unsigned $ 60)) eqn:Heqe1;
+    destruct (zlt (Int.signed $ 60) (Int.signed $ 4095)) eqn:Heqe2;
+    destruct (zeq (Int.unsigned $ 60) (Int.unsigned $ 4095)) eqn:Heqe3; eauto; tryfalse.
+Qed.
+
+Lemma get_range_0_4_stable :
+  forall id,
+    $ 0 <=ᵤᵢ id <=ᵤᵢ $ 7 -> get_range 0 4 id = id.
+Proof.
+  intros.
+  rewrite <- Int.repr_unsigned.
+  unfold get_range.
+  unfold Int.and.
+  unfold Int.shl.
+  unfold Int.sub.
+  simpl.
+  assert (Int.unsigned $ 1 = 1%Z).
+  simpl; eauto.
+  assert (Int.unsigned $ 5 = 5%Z).
+  simpl; eauto.
+  assert (Int.unsigned $ 0 = 0%Z).
+  simpl; eauto.
+  rewrite H0, H1, H2.
+  simpl.
+  assert (Int.unsigned $ 32 = 32%Z).
+  simpl; eauto.
+  rewrite H3.
+  simpl; eauto.
+  assert (Int.unsigned $ 31 = 31%Z).
+  simpl; eauto.
+  do 2 rewrite H4.
+  destruct id.
+  unfold int_leu, Int.eq, Int.ltu in H.
+  rewrite H2 in H.
+  assert (Int.unsigned $ 7 = 7%Z).
+  simpl; eauto.
+  rewrite H5 in H; eauto.
+  simpl Int.unsigned in H.
+  simpl. 
+  destruct (zlt 0 intval); destruct (zeq 0 intval);
+    destruct (zlt intval 7); destruct (zeq intval 7); simpls; tryfalse; try omega.
+  clear H H0 H1 H2 H3 H4 H5.
+  assert (Z.land intval 31 = intval).
+  {
+    unfold Z.land.
+    destruct intval; tryfalse.
+    clear - l l0.
+    repeat (destruct p; simpl; eauto; tryfalse; try omega).
+  } 
+  rewrite H.
+  eauto.
+  clear H H0 H1 H2 H3 H4 H5.
+  rewrite e; simpl; eauto. 
+  rewrite <- e; simpl; eauto. 
+Qed.
+
+Lemma and_zero_not_eq :
+  forall v1 v2,
+    $ 0 <=ᵤᵢ v1 <=ᵤᵢ $ 7 -> $ 0 <=ᵤᵢ v2 <=ᵤᵢ $ 7 ->
+    (($ 1) <<ᵢ v1) &ᵢ (($ 1) <<ᵢ v2) = $ 0 ->
+    v1 <> v2.
+Proof.
+  intros.
+  intro.
+  subst.
+  rewrite Int.and_idem in H1.
+  clear H.
+  unfolds int_leu.
+  unfolds Int.ltu, Int.eq.
+  rewrite <- Int.repr_unsigned with (i := v2) in H1.
+  destruct v2.
+  simpl Int.unsigned in H0. 
+  assert (Int.unsigned $ 0 = 0%Z).
+  simpl; eauto.
+  assert (Int.unsigned $ 7 = 7%Z).
+  simpl; eauto.
+  rewrite H in H0.
+  rewrite H2 in H0.
+  simpl in H1.
+  destruct (zlt 0 intval);
+    destruct (zeq 0 intval);
+    destruct (zlt intval 7); destruct (zeq intval 7); tryfalse; try omega.
+  {
+    clear - l l0 H1.
+    unfolds Int.shl.
+    assert (Int.unsigned $ 1 = 1%Z).
+    simpl; eauto.
+    rewrite H in H1.
+    clear H.
+    destruct intval; simpls; tryfalse; eauto.
+    destruct p; tryfalse;
+    destruct p; tryfalse;
+    destruct p; tryfalse.
+  }
+  {
+    subst.
+    unfolds Int.shl.
+    rewrite H2 in H1.
+    assert (Int.unsigned $ 1 = 1%Z).
+    simpl; eauto.
+    rewrite H3 in H1.
+    simpls.
+    tryfalse.
+  }
+  {
+    subst.
+    unfolds Int.shl.
+    assert (Int.unsigned $ 1 = 1%Z).
+    simpl; eauto.
+    rewrite H3 in H1.
+    rewrite H in H1.
+    simpls.
+    tryfalse.
+  }
+Qed.
+
+Lemma range_0_7_int_unsigned_eq :
+  forall z,
+    (0 < z)%Z ->  (z < 7)%Z ->
+    Int.unsigned $ z = z.
+Proof.
+  intros.
+  rewrite Int.unsigned_repr_eq.
+  unfold Int.modulus.
+  unfold two_power_nat.
+  simpl.
+  destruct z; tryfalse.
+  destruct p; tryfalse; eauto;
+    destruct p; tryfalse; eauto;
+      destruct p; tryfalse; eauto.
+Qed.
+
+Lemma range_0_7_shiftl_int_unsigned_eq :
+  forall z,
+    (0 < z)%Z ->  (z < 7)%Z ->
+    Int.unsigned $ (Z.shiftl 1 z) = Z.shiftl 1 z.
+Proof.
+  intros.
+  rewrite Int.unsigned_repr_eq.
+  unfold Int.modulus.
+  unfold two_power_nat.
+  simpl.
+  destruct z; tryfalse.
+  destruct p; tryfalse; eauto;
+    destruct p; tryfalse; eauto;
+      destruct p; tryfalse; eauto.
+Qed.
+
+Lemma range_0_7_add_7_eq :
+  forall z,
+    (0 < z)%Z ->  (z < 7)%Z ->
+    Int.unsigned $ (z + 7) = (z + 7)%Z.
+Proof.
+  intros.
+  rewrite Int.unsigned_repr_eq.
+  unfold Int.modulus.
+  unfold two_power_nat.
+  simpl.
+  destruct z; tryfalse.
+  destruct p; tryfalse; eauto;
+    destruct p; tryfalse; eauto;
+      destruct p; tryfalse; eauto.
+Qed.
+
+Lemma range_0_7_add_8_eq :
+  forall z,
+    (0 < z)%Z ->  (z < 7)%Z ->
+    Int.unsigned $ (z + 8) = (z + 8)%Z.
+Proof.
+  intros.
+  rewrite Int.unsigned_repr_eq.
+  unfold Int.modulus.
+  unfold two_power_nat.
+  simpl.
+  destruct z; tryfalse.
+  destruct p; tryfalse; eauto;
+    destruct p; tryfalse; eauto;
+      destruct p; tryfalse; eauto.
+Qed.
+
+Lemma and_not_zero_eq :
+  forall v1 v2,
+    $ 0 <=ᵤᵢ v1 <=ᵤᵢ $ 7 -> $ 0 <=ᵤᵢ v2 <=ᵤᵢ $ 7 ->
+    (($ 1) <<ᵢ v1) &ᵢ (($ 1) <<ᵢ v2) <> $ 0 ->
+    v1 = v2.
+Proof.
+  intros.
+  rewrite <- Int.repr_unsigned with (i := v1).
+  rewrite <- Int.repr_unsigned with (i := v2).
+  rewrite <- Int.repr_unsigned with (i := v1) in H1.
+  rewrite <- Int.repr_unsigned with (i := v2) in H1.
+  unfolds int_leu.
+  unfolds Int.ltu.
+  unfolds Int.eq.
+  assert (Int.unsigned $ 0 = 0%Z).
+  simpl; eauto.
+  assert (Int.unsigned $ 7 = 7%Z).
+  simpl; eauto.
+  try rewrite H2 in *.
+  try rewrite H3 in *.
+  destruct v1, v2.
+  simpl Int.unsigned in *.
+  unfolds Int.shl.
+  assert (Int.unsigned $ 1 = 1%Z).
+  simpl; eauto.
+  try rewrite H4 in *.
+  unfold Int.and in H1.
+  destruct (zlt 0 intval);
+    destruct (zeq 0 intval); destruct (zlt intval 7); destruct (zeq intval 7);
+      destruct (zlt 0 intval0);
+      destruct (zeq 0 intval0); destruct (zlt intval0 7); destruct (zeq intval0 7);
+        tryfalse; simpls; subst; eauto; try omega.
+  {
+    rewrite range_0_7_int_unsigned_eq with (z := intval) in H1; eauto.
+    rewrite range_0_7_int_unsigned_eq with (z := intval0) in H1; eauto.
+    rewrite range_0_7_shiftl_int_unsigned_eq in H1; eauto.
+    rewrite range_0_7_shiftl_int_unsigned_eq in H1; eauto.
+    
+    destruct intval, intval0; simpl; eauto; try omega; tryfalse.
+    destruct p; destruct p0;
+      try destruct p; try destruct p0;
+        try destruct p; try destruct p0; tryfalse; simpl; eauto; simpls; tryfalse;
+          try solve [unfolds Int.unsigned; simpls; tryfalse].
+  }
+  {
+    rewrite range_0_7_int_unsigned_eq with (z := intval) in H1; eauto.
+    rewrite range_0_7_shiftl_int_unsigned_eq in H1; eauto.
+    rewrite H3 in H1.
+    simpl in H1.
+    assert (Int.unsigned $ 128 = 128%Z).
+    eauto.
+    rewrite H5 in H1.
+
+    destruct intval; simpl; eauto; try omega; tryfalse.
+    destruct p; try destruct p; try destruct p;
+      tryfalse; simpl; eauto; simpls; tryfalse.
+  }
+  {
+    rewrite range_0_7_int_unsigned_eq with (z := intval) in H1; eauto.
+    rewrite range_0_7_shiftl_int_unsigned_eq in H1; eauto.
+    rewrite H2 in H1.
+    simpl in H1.
+    rewrite H4 in H1.
+
+    destruct intval; simpl; eauto; try omega; tryfalse.
+    destruct p; try destruct p; try destruct p;
+      tryfalse; simpl; eauto; simpls; tryfalse.
+  }
+  { 
+    rewrite range_0_7_int_unsigned_eq with (z := intval0) in H1; eauto.
+    rewrite H3 in H1.
+    simpl in H1.
+    assert (Int.unsigned $ 128 = 128%Z).
+    eauto.
+    rewrite H5 in H1.
+    rewrite range_0_7_shiftl_int_unsigned_eq in H1; eauto.
+
+    destruct intval0; simpl; eauto; try omega; tryfalse.
+    destruct p; try destruct p; try destruct p;
+      tryfalse; simpl; eauto; simpls; tryfalse.
+  }
+  {
+    rewrite H3 in H1.
+    rewrite H2 in H1.
+    simpls.
+    assert (Int.unsigned $ 128 = 128%Z).
+    eauto.
+    rewrite H5 in H1.
+    rewrite H4 in H1.
+    simpls.
+    tryfalse.
+  }
+  {
+    rewrite range_0_7_int_unsigned_eq with (z := intval0) in H1; eauto.
+    rewrite H2 in H1.
+    simpl in H1.
+    rewrite H4 in H1.
+    rewrite range_0_7_shiftl_int_unsigned_eq in H1; eauto.
+
+    destruct intval0; simpl; eauto; try omega; tryfalse.
+    destruct p; try destruct p; try destruct p;
+      tryfalse; simpl; eauto; simpls; tryfalse.
+  }
+  {
+    rewrite H3 in H1.
+    rewrite H2 in H1.
+    simpls.
+    rewrite H4 in H1.
+    assert (Int.unsigned $ 128 = 128%Z).
+    eauto.
+    rewrite H5 in H1.
+    simpls.
+    tryfalse.
+  }
+Qed.
+
+Lemma in_range_0_7_pre_cwp_still :
+  forall id,
+    $ 0 <=ᵤᵢ id <=ᵤᵢ $ 7 ->
+    $ 0 <=ᵤᵢ (pre_cwp id) <=ᵤᵢ $ 7.
+Proof.
+  intros.
+  unfold pre_cwp.
+  unfolds int_leu.
+  unfolds Int.ltu.
+  unfolds Int.eq.
+  unfold N.
+  unfold Int.add.
+  unfold Int.sub.
+  assert (Int.unsigned $ 0 = 0%Z).
+  eauto.
+  assert (Int.unsigned $ 7 = 7%Z).
+  eauto.
+  assert (Int.unsigned $ 8 = 8%Z).
+  eauto.
+  assert (Int.unsigned $ 1 = 1%Z).
+  eauto.
+  try rewrite H0 in *.
+  try rewrite H1 in *.
+  try rewrite H2 in *.
+  try rewrite H3 in *.
+  destruct id.
+  simpl Int.unsigned in *.
+  destruct (zlt 0 intval);
+    destruct (zeq 0 intval); destruct (zlt intval 7); destruct (zeq intval 7);
+      eauto; tryfalse; try omega.
+  {
+    destruct intval; eauto; tryfalse.
+    destruct p;
+      try destruct p; try destruct p; tryfalse; try omega; eauto.
+  }
+  {
+    subst.
+    eauto.
+  }
+  {
+    subst.
+    eauto.
+  }
+Qed.
+
+Lemma in_range_0_7_post_cwp_still :
+  forall id,
+    $ 0 <=ᵤᵢ id <=ᵤᵢ $ 7 ->
+    $ 0 <=ᵤᵢ (post_cwp id) <=ᵤᵢ $ 7.
+Proof.
+  intros.
+  unfold post_cwp.
+  unfolds int_leu.
+  unfolds Int.ltu.
+  unfolds Int.eq.
+  unfold N.
+  unfold Int.add.
+  unfold Int.sub.
+  assert (Int.unsigned $ 0 = 0%Z).
+  eauto.
+  assert (Int.unsigned $ 7 = 7%Z).
+  eauto.
+  assert (Int.unsigned $ 8 = 8%Z).
+  eauto.
+  assert (Int.unsigned $ 1 = 1%Z).
+  eauto.
+  try rewrite H0 in *.
+  try rewrite H1 in *.
+  try rewrite H2 in *.
+  try rewrite H3 in *.
+  destruct id.
+  simpl Int.unsigned in *.
+  destruct (zlt 0 intval);
+    destruct (zeq 0 intval); destruct (zlt intval 7); destruct (zeq intval 7);
+      eauto; tryfalse; try omega.
+  {
+    destruct intval; eauto; tryfalse.
+    destruct p;
+      try destruct p; try destruct p; tryfalse; try omega; eauto.
+  }
+  {
+    subst.
+    eauto.
+  }
+  {
+    subst.
+    eauto.
+  }
+Qed.
+
+Lemma win_mask_pre_cwp :
+  forall id,
+    $ 0 <=ᵤᵢ id <=ᵤᵢ $ 7 ->
+    (($ 1) <<ᵢ (pre_cwp id)) &ᵢ (($ 1) <<ᵢ id) = $ 0.
+Proof.
+  intros.
+  unfolds int_leu.
+  unfolds Int.ltu.
+  unfolds Int.eq.
+  assert (Int.unsigned $ 0 = 0%Z).
+  eauto.
+  assert (Int.unsigned $ 7 = 7%Z).
+  eauto.
+  assert (Int.unsigned $ 1 = 1%Z).
+  eauto.
+  assert (Int.unsigned $ 8 = 8%Z).
+  eauto.
+  unfold pre_cwp.
+  unfold Int.and.
+  unfold Int.shl.
+  unfold Int.add.
+  unfold Int.sub.
+  unfold N.
+  try rewrite H0 in *.
+  try rewrite H1 in *.
+  try rewrite H2 in *.
+  try rewrite H3 in *.
+  destruct id.
+  simpl Int.unsigned in *.
+  destruct (zlt 0 intval); destruct (zeq 0 intval);
+    destruct (zlt intval 7); destruct (zeq intval 7); tryfalse; try omega.
+  {
+    rewrite range_0_7_add_8_eq; eauto.
+    assert ((intval + 8 - 1 = intval + 7)%Z).
+    omega.
+    rewrite H4.
+    unfold Int.modu.
+    rewrite H3.
+    destruct intval; eauto; tryfalse.
+    do 3 (try destruct p; eauto; tryfalse).
+  }
+  {
+    subst.
+    unfold Int.modu.
+    simpl.
+    rewrite H3.
+    eauto.
+  }
+  {
+    subst.
+    unfold Int.modu.
+    rewrite H3.
+    simpl.
+    eauto.
+  }
+Qed.
+
+Lemma post_1_neq :
+  forall id,
+    $ 0 <=ᵤᵢ id <=ᵤᵢ $ 7 ->
+    post_cwp id <> id.
+Proof.
+  intros.
+  intro.
+  rewrite <- Int.repr_unsigned with (i := id) in H0.
+  unfolds post_cwp.
+  unfolds int_leu.
+  unfolds Int.ltu, Int.eq.
+  unfolds Int.add.
+  unfolds Int.modu.
+  unfolds N.
+  assert (Int.unsigned $ 0 = 0%Z); eauto.
+  assert (Int.unsigned $ 7 = 7%Z); eauto.
+  assert (Int.unsigned $ 1 = 1%Z); eauto.
+  assert (Int.unsigned $ 8 = 8%Z); eauto.
+  try rewrite H1 in *.
+  try rewrite H2 in *.
+  try rewrite H3 in *.
+  try rewrite H4 in *.
+  destruct id.
+  simpl Int.unsigned in *.
+  destruct (zlt 0 intval); destruct (zeq 0 intval);
+    destruct (zlt intval 7); destruct (zeq intval 7); tryfalse; try omega.
+  {
+    destruct intval; eauto; tryfalse.
+    do 3 (try destruct p; simpls; tryfalse; try omega).
+  }
+  {
+    subst.
+    rewrite H2 in H0.
+    simpls; eauto.
+    tryfalse.
+  }
+  {
+    subst.
+    rewrite H1 in H0.
+    simpls; eauto.
+    tryfalse.
+  }
+Qed.
+
+Lemma post_2_neq :
+  forall id,
+    $ 0 <=ᵤᵢ id <=ᵤᵢ $ 7 ->
+    post_cwp (post_cwp id) <> id.
+Proof.
+  intros.
+  intro.
+  rewrite <- Int.repr_unsigned with (i := id) in H0.
+  unfolds post_cwp.
+  unfolds int_leu.
+  unfolds Int.ltu, Int.eq.
+  unfolds Int.add.
+  unfolds Int.modu.
+  unfolds N.
+  assert (Int.unsigned $ 0 = 0%Z); eauto.
+  assert (Int.unsigned $ 7 = 7%Z); eauto.
+  assert (Int.unsigned $ 1 = 1%Z); eauto.
+  assert (Int.unsigned $ 8 = 8%Z); eauto.
+  try rewrite H1 in *.
+  try rewrite H2 in *.
+  try rewrite H3 in *.
+  try rewrite H4 in *.
+  destruct id.
+  simpl Int.unsigned in *.
+  destruct (zlt 0 intval); destruct (zeq 0 intval);
+    destruct (zlt intval 7); destruct (zeq intval 7); tryfalse; try omega.
+  { 
+    destruct intval; eauto; tryfalse.
+    do 3 (try destruct p; simpls; tryfalse; try omega).
+  }
+  {
+    subst.
+    rewrite H2 in H0.
+    simpls; eauto.
+    tryfalse.
+  }
+  {
+    subst.
+    rewrite H1 in H0.
+    simpls; eauto.
+    tryfalse.
+  }
+Qed.
+
+Lemma post_3_neq :
+  forall id,
+    $ 0 <=ᵤᵢ id <=ᵤᵢ $ 7 ->
+    post_cwp (post_cwp (post_cwp id)) <> id.
+Proof.
+  intros.
+  intro.
+  rewrite <- Int.repr_unsigned with (i := id) in H0.
+  unfolds post_cwp.
+  unfolds int_leu.
+  unfolds Int.ltu, Int.eq.
+  unfolds Int.add.
+  unfolds Int.modu.
+  unfolds N.
+  assert (Int.unsigned $ 0 = 0%Z); eauto.
+  assert (Int.unsigned $ 7 = 7%Z); eauto.
+  assert (Int.unsigned $ 1 = 1%Z); eauto.
+  assert (Int.unsigned $ 8 = 8%Z); eauto.
+  try rewrite H1 in *.
+  try rewrite H2 in *.
+  try rewrite H3 in *.
+  try rewrite H4 in *.
+  destruct id.
+  simpl Int.unsigned in *.
+  destruct (zlt 0 intval); destruct (zeq 0 intval);
+    destruct (zlt intval 7); destruct (zeq intval 7); tryfalse; try omega.
+  {
+    destruct intval; eauto; tryfalse.
+    do 3 (try destruct p; simpls; tryfalse; try omega).
+  }
+  {
+    subst.
+    rewrite H2 in H0.
+    simpls; eauto.
+    tryfalse.
+  }
+  {
+    subst.
+    rewrite H1 in H0.
+    simpls; eauto.
+    tryfalse.
+  }
+Qed.
+
+Lemma post_4_neq :
+  forall id,
+    $ 0 <=ᵤᵢ id <=ᵤᵢ $ 7 ->
+    post_cwp (post_cwp (post_cwp (post_cwp id))) <> id.
+Proof.
+  intros.
+  intro.
+  rewrite <- Int.repr_unsigned with (i := id) in H0.
+  unfolds post_cwp.
+  unfolds int_leu.
+  unfolds Int.ltu, Int.eq.
+  unfolds Int.add.
+  unfolds Int.modu.
+  unfolds N.
+  assert (Int.unsigned $ 0 = 0%Z); eauto.
+  assert (Int.unsigned $ 7 = 7%Z); eauto.
+  assert (Int.unsigned $ 1 = 1%Z); eauto.
+  assert (Int.unsigned $ 8 = 8%Z); eauto.
+  try rewrite H1 in *.
+  try rewrite H2 in *.
+  try rewrite H3 in *.
+  try rewrite H4 in *.
+  destruct id.
+  simpl Int.unsigned in *.
+  destruct (zlt 0 intval); destruct (zeq 0 intval);
+    destruct (zlt intval 7); destruct (zeq intval 7); tryfalse; try omega.
+  {
+    destruct intval; eauto; tryfalse.
+    do 3 (try destruct p; simpls; tryfalse; try omega).
+  }
+  {
+    subst.
+    rewrite H2 in H0.
+    simpls; eauto.
+    tryfalse.
+  }
+  {
+    subst.
+    rewrite H1 in H0.
+    simpls; eauto.
+    tryfalse.
+  }
+Qed.
+
+Lemma post_5_neq :
+  forall id,
+    $ 0 <=ᵤᵢ id <=ᵤᵢ $ 7 ->
+    post_cwp (post_cwp (post_cwp (post_cwp (post_cwp id)))) <> id.
+Proof.
+  intros.
+  intro.
+  rewrite <- Int.repr_unsigned with (i := id) in H0.
+  unfolds post_cwp.
+  unfolds int_leu.
+  unfolds Int.ltu, Int.eq.
+  unfolds Int.add.
+  unfolds Int.modu.
+  unfolds N.
+  assert (Int.unsigned $ 0 = 0%Z); eauto.
+  assert (Int.unsigned $ 7 = 7%Z); eauto.
+  assert (Int.unsigned $ 1 = 1%Z); eauto.
+  assert (Int.unsigned $ 8 = 8%Z); eauto.
+  try rewrite H1 in *.
+  try rewrite H2 in *.
+  try rewrite H3 in *.
+  try rewrite H4 in *.
+  destruct id.
+  simpl Int.unsigned in *.
+  destruct (zlt 0 intval); destruct (zeq 0 intval);
+    destruct (zlt intval 7); destruct (zeq intval 7); tryfalse; try omega.
+  {
+    destruct intval; eauto; tryfalse.
+    do 3 (try destruct p; simpls; tryfalse; try omega).
+  }
+  {
+    subst.
+    rewrite H2 in H0.
+    simpls; eauto.
+    tryfalse.
+  }
+  {
+    subst.
+    rewrite H1 in H0.
+    simpls; eauto.
+    tryfalse.
+  }
+Qed.
+
+Lemma post_6_neq :
+  forall id,
+    $ 0 <=ᵤᵢ id <=ᵤᵢ $ 7 ->
+    post_cwp (post_cwp (post_cwp (post_cwp (post_cwp (post_cwp id))))) <> id.
+Proof.
+  intros.
+  intro.
+  rewrite <- Int.repr_unsigned with (i := id) in H0.
+  unfolds post_cwp.
+  unfolds int_leu.
+  unfolds Int.ltu, Int.eq.
+  unfolds Int.add.
+  unfolds Int.modu.
+  unfolds N.
+  assert (Int.unsigned $ 0 = 0%Z); eauto.
+  assert (Int.unsigned $ 7 = 7%Z); eauto.
+  assert (Int.unsigned $ 1 = 1%Z); eauto.
+  assert (Int.unsigned $ 8 = 8%Z); eauto.
+  try rewrite H1 in *.
+  try rewrite H2 in *.
+  try rewrite H3 in *.
+  try rewrite H4 in *.
+  destruct id.
+  simpl Int.unsigned in *.
+  destruct (zlt 0 intval); destruct (zeq 0 intval);
+    destruct (zlt intval 7); destruct (zeq intval 7); tryfalse; try omega.
+  {
+    destruct intval; eauto; tryfalse.
+    do 3 (try destruct p; simpls; tryfalse; try omega).
+  }
+  {
+    subst.
+    rewrite H2 in H0.
+    simpls; eauto.
+    tryfalse.
+  }
+  {
+    subst.
+    rewrite H1 in H0.
+    simpls; eauto.
+    tryfalse.
+  }
+Qed.
+
+Lemma post_7_eq :
+  forall id,
+    $ 0 <=ᵤᵢ id <=ᵤᵢ $ 7 ->
+    post_cwp (post_cwp (post_cwp (post_cwp (post_cwp (post_cwp (post_cwp id)))))) <> id.
+Proof.
+  intros.
+  intro.
+  rewrite <- Int.repr_unsigned with (i := id) in H0.
+  unfolds post_cwp.
+  unfolds int_leu.
+  unfolds Int.ltu, Int.eq.
+  unfolds Int.add.
+  unfolds Int.modu.
+  unfolds N.
+  assert (Int.unsigned $ 0 = 0%Z); eauto.
+  assert (Int.unsigned $ 7 = 7%Z); eauto.
+  assert (Int.unsigned $ 1 = 1%Z); eauto.
+  assert (Int.unsigned $ 8 = 8%Z); eauto.
+  try rewrite H1 in *.
+  try rewrite H2 in *.
+  try rewrite H3 in *.
+  try rewrite H4 in *.
+  destruct id.
+  simpl Int.unsigned in *.
+  destruct (zlt 0 intval); destruct (zeq 0 intval);
+    destruct (zlt intval 7); destruct (zeq intval 7); tryfalse; try omega.
+  {
+    destruct intval; eauto; tryfalse.
+    do 3 (try destruct p; simpls; tryfalse; try omega).
+  }
+  {
+    subst.
+    rewrite H2 in H0.
+    simpls; eauto.
+    tryfalse.
+  }
+  {
+    subst.
+    rewrite H1 in H0.
+    simpls; eauto.
+    tryfalse.
+  }
+Qed.
+
+Lemma post_8_eq :
+  forall id,
+    $ 0 <=ᵤᵢ id <=ᵤᵢ $ 7 ->
+    post_cwp (post_cwp (post_cwp (post_cwp (post_cwp (post_cwp (post_cwp (post_cwp id))))))) = id.
+Proof.
+  intros.
+  rewrite <- Int.repr_unsigned with (i := id).
+  unfolds post_cwp.
+  unfolds int_leu.
+  unfolds Int.ltu, Int.eq.
+  unfolds Int.add.
+  unfolds Int.modu.
+  unfolds N.
+  assert (Int.unsigned $ 0 = 0%Z); eauto.
+  assert (Int.unsigned $ 7 = 7%Z); eauto.
+  assert (Int.unsigned $ 1 = 1%Z); eauto.
+  assert (Int.unsigned $ 8 = 8%Z); eauto.
+  try rewrite H0 in *.
+  try rewrite H1 in *.
+  try rewrite H2 in *.
+  try rewrite H3 in *. 
+  destruct id.
+  simpl Int.unsigned in *. 
+  destruct (zlt 0 intval); destruct (zeq 0 intval);
+    destruct (zlt intval 7); destruct (zeq intval 7); tryfalse; try omega; eauto.
+  {
+    destruct intval; eauto; tryfalse.
+    do 3 (try destruct p; tryfalse; try omega; eauto).
+  }
+  {
+    subst.
+    eauto.
+  }
+  {
+    subst.
+    eauto.
+  }
+Qed.
+
+Lemma set_wim_eq_pre_cwp :
+  forall id,
+    $ 0 <=ᵤᵢ id <=ᵤᵢ $ 7 ->
+    get_range 0 7 ((($ 1) <<ᵢ id) <<ᵢ ($ 7)) |ᵢ ((($ 1) <<ᵢ id) >>ᵢ ($ 1)) =
+                                              ($ 1) <<ᵢ (pre_cwp id).
+Proof.
+  intros.
+  unfold get_range.
+  unfold pre_cwp.
+  unfolds int_leu.
+  unfolds Int.ltu, Int.eq.
+  unfold Int.shl.
+  unfold Int.shru.
+  unfold Int.add.
+  unfold Int.sub.
+  unfold N.
+  simpl.
+  assert (Int.unsigned $ 0 = 0%Z).
+  eauto.
+  assert (Int.unsigned $ 1 = 1%Z).
+  eauto.
+  assert (Int.unsigned $ 7 = 7%Z).
+  eauto.
+  assert (Int.unsigned $ 8 = 8%Z).
+  eauto.
+  try rewrite H0 in *.
+  try rewrite H1 in *.
+  try rewrite H2 in *.
+  try rewrite H3 in *.
+  destruct id. 
+  simpls Int.unsigned.
+  unfold Int.modu, Int.or, Int.and.
+  rewrite H3.
+  destruct (zlt 0 intval); destruct (zeq 0 intval);
+    destruct (zlt intval 7); destruct (zeq intval 7);
+      tryfalse; try omega; eauto.
+  {
+    destruct intval; tryfalse.
+    do 3 (try destruct p; eauto; tryfalse).
+  }
+  {
+    subst; eauto.
+  }
+  {
+    subst; eauto.
+  }
+Qed.
+
+Lemma post_pre_stable :
+  forall id,
+    $ 0 <=ᵤᵢ id <=ᵤᵢ $ 7 ->
+    post_cwp (pre_cwp id) = id.
+Proof.
+  intros.
+  rewrite <- Int.repr_unsigned.
+  unfolds int_leu.
+  unfolds Int.ltu, Int.eq.
+  unfold post_cwp.
+  unfold pre_cwp.
+  unfold N.
+  unfold Int.add.
+  unfold Int.sub.
+  unfold Int.modu.
+  assert (Int.unsigned $ 0 = 0%Z).
+  eauto.
+  assert (Int.unsigned $ 7 = 7%Z).
+  eauto.
+  assert (Int.unsigned $ 8 = 8%Z).
+  eauto.
+  assert (Int.unsigned $ 1 = 1%Z).
+  eauto.
+  try rewrite H0 in *.
+  try rewrite H1 in *.
+  try rewrite H2 in *.
+  try rewrite H3 in *.
+  destruct id.
+  simpl Int.unsigned in *.
+  destruct (zlt 0 intval); destruct (zeq 0 intval);
+    destruct (zlt intval 7); destruct (zeq intval 7); tryfalse; try omega;
+      subst; eauto.
+  destruct intval; tryfalse.
+  do 3 (destruct p; tryfalse; eauto).
+Qed.
