coqimp/contextswitch/lib/tm_dly_lemma.v
@@ -1,0 +1,438 @@
+Require Import Coqlib.                         
+Require Import Maps.           
+Require Import LibTactics.   
+        
+Require Import Integers.  
+Open Scope Z_scope.        
+Import ListNotations.  
+   
+Set Asymmetric Patterns.  
+        
+Require Import state.    
+Require Import language. 
+ 
+Set Implicit Arguments.    
+Unset Strict Implicit. 
+               
+Require Import logic.
+    
+Require Import lemmas.
+Require Import lemmas_ins.
+
+Require Import Coq.Logic.FunctionalExtensionality.
+
+Require Import sep_lemma.
+Require Import reg_lemma.
+
+Require Import ctxswitch_spec.
+
+Open Scope nat.
+Open Scope code_scope.
+Open Scope mem_scope.
+
+(*+ Lemmas about TimReduce +*)
+Theorem astar_TimReduce :
+  forall p q,
+    (p ** q) ↓ = (p ↓) ** (q ↓).
+Proof.
+  intros; simpl; eauto.
+Qed.
+
+Theorem GenRegs_TimeReduce :
+  forall grst p,
+    (GenRegs grst ** p) ↓ = GenRegs grst ** (p ↓).
+Proof.
+  intros.
+  simpl.
+  destruct grst.
+  destruct p0.
+  destruct p0.
+  destruct f1, f2, f0, f.
+  simpl.
+  eauto.
+Qed.
+
+Theorem FrameState_TimeReduce :
+  forall id vi F p,
+    (FrameState id vi F ** p) ↓ = FrameState id vi F ** (p ↓).
+Proof.
+  intros.
+  simpls.
+  unfold FrameState.
+  eauto.
+Qed.
+
+Theorem RegSt_TimeReduce :
+  forall rn v p,
+    (rn |=> v ** p) ↓ = rn |=> v ** (p ↓).
+Proof.
+  intros.
+  simpl; eauto.
+Qed.
+
+Theorem MemSto_TimeReduce :
+  forall l v p,
+    (l |-> v ** p) ↓ = l |-> v ** (p ↓).
+Proof.
+  intros.
+  simpl; eauto.
+Qed.
+
+Lemma save_reg_TimeReduce' :
+  forall n l vl,
+    save_reg l n vl ↓ = save_reg l n vl.
+Proof.
+  intro n.
+  induction n; intros.
+  -
+    simpls.
+    destruct vl; eauto.
+  -
+    destruct vl.
+    {
+      simpl.
+      eauto.
+    }
+    {
+      simpl.
+      rewrite IHn; eauto.
+    }
+Qed.
+
+Lemma save_reg_TimeReduce :
+  forall n l vl p,
+    (save_reg l n vl ** p) ↓ = save_reg l n vl ** (p ↓).
+Proof.
+  intros.
+  simpl.
+  rewrite save_reg_TimeReduce'; eauto.
+Qed.
+
+Theorem Context_TimeReduce' :
+  forall ctx,
+    (context ctx) ↓ = context ctx.
+Proof.
+  intros.
+  unfold context.
+  destruct ctx.
+  destruct p.
+  destruct p.
+  destruct p.
+  unfold context'.
+  repeat (rewrite save_reg_TimeReduce; eauto).
+Qed.
+
+Theorem Context_TimeReduce :
+  forall ctx p,
+    (context ctx ** p) ↓ = context ctx ** (p ↓).
+Proof.
+  intros.
+  simpls.
+  unfold context.
+  destruct ctx.
+  destruct p0.
+  destruct p0.
+  destruct p0.
+  unfold context'.
+  do 3 rewrite save_reg_TimeReduce.
+  simpl; eauto.
+Qed.
+
+Lemma stack_seg_TimeReduce :
+  forall l fm,
+    stack_seg l fm ↓ = stack_seg l fm.
+Proof.
+  intros.
+  destruct fm.
+  unfold stack_seg.
+  simpl; eauto.
+Qed.
+
+Lemma stack_frame_TimeReduce :
+  forall l fm1 fm2,
+    stack_frame l fm1 fm2 ↓ = stack_frame l fm1 fm2.
+Proof.
+  intros.
+  unfold stack_frame.
+  rewrite astar_TimReduce.
+  do 2 rewrite stack_seg_TimeReduce.
+  simpl; eauto.
+Qed.
+
+Lemma Stk_TimeReduce' :
+  forall lfp l,
+    stack' l lfp ↓ = stack' l lfp.
+Proof.
+  intro lfp.
+  induction lfp; intros.
+  -
+    simpl; eauto.
+  -
+    simpl. 
+    destruct a.
+    simpl.
+    do 2 rewrite stack_seg_TimeReduce; eauto.
+    rewrite IHlfp; eauto.
+Qed.
+
+Lemma Stk_TimeReduce1 :
+  forall stk,
+    stack stk ↓ = stack stk.
+Proof.
+  intros.
+  unfold stack.
+  destruct stk.
+  rewrite Stk_TimeReduce'; eauto.
+Qed.
+
+Theorem Stk_TimeReduce :
+  forall stk p,
+    (stack stk ** p) ↓ = stack stk ** (p ↓).
+Proof.
+  intros.
+  destruct stk.
+  unfold stack.
+  simpl.
+  rewrite Stk_TimeReduce'; eauto.
+Qed.
+
+Theorem conj_TimeReduce :
+  forall p1 p2,
+    (p1 //\\ p2) ↓ = (p1 ↓) //\\ (p2 ↓).
+Proof.
+  intros; eauto.
+Qed.
+
+Theorem disj_TimeReduce :
+  forall p1 p2,
+    (p1 \\// p2) ↓ = (p1 ↓) \\// (p2 ↓).
+Proof.
+  intros; eauto.
+Qed.
+
+Theorem pure_TimeReduce :
+  forall pu p,
+    ([| pu |] ** p) ↓ = [| pu |] ** (p ↓).
+Proof.
+  intros; eauto.
+Qed.
+
+Theorem Atrue_TimeReduce :
+  forall p,
+    (Atrue ** p) ↓ = Atrue ** (p ↓).
+Proof.
+  intros; eauto.
+Qed.
+
+Theorem Afalse_TimReduce :
+  forall p,
+    (Afalse ** p) ↓ = Afalse ** (p ↓).
+Proof.
+  intros; eauto.
+Qed.
+
+Ltac TimReduce_simpl :=
+  match goal with
+  | |- context [(context ?ctx) ↓] =>
+    rewrite Context_TimeReduce'; TimReduce_simpl
+  | |- context [(stack ?stk) ↓] =>
+    rewrite Stk_TimeReduce1; TimReduce_simpl
+  | |- context [(GenRegs ?grst ** ?p) ↓] =>
+    rewrite GenRegs_TimeReduce; TimReduce_simpl
+  | |- context [(FrameState ?id ?vi ?F ** ?p) ↓] =>
+    rewrite FrameState_TimeReduce; TimReduce_simpl
+  | |- context [(?rn |=> ?v ** ?p) ↓] =>
+    rewrite RegSt_TimeReduce; TimReduce_simpl
+  | |- context [(?l |-> ?v ** ?p) ↓] =>
+    rewrite MemSto_TimeReduce; TimReduce_simpl
+  | |- context [(context ?ctx ** ?p) ↓] =>
+    rewrite Context_TimeReduce; TimReduce_simpl
+  | |- context [(stack ?stk ** ?p) ↓] =>
+    rewrite Stk_TimeReduce; TimReduce_simpl
+  | |- context [([| ?pu |] ** ?p) ↓] =>
+    rewrite pure_TimeReduce; TimReduce_simpl
+  | |- context [(Atrue ** ?p) ↓] =>
+    rewrite Atrue_TimeReduce; TimReduce_simpl
+  | |- context [(Afalse ** ?p) ↓] =>
+    rewrite Afalse_TimReduce; TimReduce_simpl
+  | |- context [(stack' _ _) ↓] =>
+    rewrite Stk_TimeReduce'; TimReduce_simpl
+  | |- context [(stack_frame _ _ _) ↓] =>
+    rewrite stack_frame_TimeReduce; TimReduce_simpl
+  | |- context [(?p1 //\\ ?p2) ↓] =>
+    rewrite conj_TimeReduce; TimReduce_simpl
+  | |- context [(?p1 \\// ?p2) ↓] =>
+    rewrite disj_TimeReduce; TimReduce_simpl
+  | |- context [(?p1 ** ?p2) ↓] =>
+    rewrite astar_TimReduce; TimReduce_simpl
+  | _ => simpl TimReduce
+  end.
+
+Ltac TimReduce_simpl_in H :=
+  match type of H with
+  | _ |= ?p =>
+    match p with
+    | context [(GenRegs ?grst ** ?p) ↓] =>
+      rewrite GenRegs_TimeReduce in H; TimReduce_simpl_in H
+    | context [(FrameState ?id ?vi ?F ** ?p) ↓] =>
+      rewrite FrameState_TimeReduce in H; TimReduce_simpl_in H
+    | context [(?rn |=> ?v ** ?p) ↓] =>
+      rewrite RegSt_TimeReduce in H; TimReduce_simpl_in H
+    | context [(?l |-> ?v ** ?p) ↓] =>
+      rewrite MemSto_TimeReduce in H; TimReduce_simpl_in H
+    | context [(context ?ctx ** ?p) ↓] =>
+      rewrite Context_TimeReduce in H; TimReduce_simpl_in H
+    | context [(stack ?stk ** ?p) ↓] =>
+      rewrite Stk_TimeReduce in H; TimReduce_simpl_in H
+    | context [([| ?pu |] ** ?p) ↓] =>
+      rewrite pure_TimeReduce in H; TimReduce_simpl_in H
+    | context [(Atrue ** ?p) ↓] =>
+      rewrite Atrue_TimeReduce in H; TimReduce_simpl_in H
+    | context [(Afalse ** ?p) ↓] =>
+      rewrite Afalse_TimReduce in H; TimReduce_simpl_in H
+    | context [(?p1 //\\ ?p2) ↓] =>
+      rewrite conj_TimeReduce in H; TimReduce_simpl_in H
+    | context [(?p1 \\// ?p2) ↓] =>
+      rewrite disj_TimeReduce in H; TimReduce_simpl_in H
+    | _ => simpl TimReduce in H
+    end
+  end.
+
+(*+ Lemmas about DlyFrameFree +*)
+Lemma Atrue_DlyFrameFree :
+  forall p,
+    DlyFrameFree p -> DlyFrameFree (Atrue ** p).
+Proof.
+  intros.
+  simpl; eauto.
+Qed.
+
+Lemma Afalse_DlyFrameFree :
+  forall p,
+    DlyFrameFree p -> DlyFrameFree (Afalse ** p).
+Proof.
+  intros.
+  simpl; eauto.
+Qed.
+
+Lemma RegSt_DlyFrameFree :
+  forall rn v p,
+    DlyFrameFree p -> DlyFrameFree (rn |=> v ** p).
+Proof.
+  intros.
+  simpl; eauto.
+Qed.
+
+Lemma MapSto_DlyFrameFree :
+  forall l v p,
+    DlyFrameFree p -> DlyFrameFree (l |-> v ** p).
+Proof.
+  intros.
+  simpl; eauto.
+Qed.
+
+Lemma astar_DlyFrameFree :
+  forall p1 p2,
+    DlyFrameFree p1 -> DlyFrameFree p2 -> DlyFrameFree (p1 ** p2).
+Proof.
+  intros.
+  simpl; eauto.
+Qed.
+
+Lemma save_reg_DlyFrameFree' :
+  forall n l vl,
+    DlyFrameFree (save_reg l n vl).
+Proof.
+  intro n.
+  induction n; intros.
+  -
+    simpls; eauto.
+    destruct vl; eauto.
+    simpl; eauto.
+    simpl; eauto.
+  -
+    destruct vl; simpl; eauto.
+Qed.
+  
+Lemma save_reg_DlyFrameFree :
+  forall n l vl p,
+    DlyFrameFree p ->
+    DlyFrameFree (save_reg l n vl ** p).
+Proof.
+  intros.
+  eapply astar_DlyFrameFree; eauto.
+  eapply save_reg_DlyFrameFree'.
+Qed.
+
+Lemma Context_DlyFrameFree' :
+  forall l rl ri rg ry,
+    DlyFrameFree (context' l rl ri rg ry).
+Proof.
+  intros.
+  unfold context'.
+  do 3 (eapply save_reg_DlyFrameFree; eauto).
+  simpl; eauto.
+Qed.
+
+Lemma Context_DlyFrameFree :
+  forall ctx p,
+    DlyFrameFree p -> DlyFrameFree (context ctx ** p).
+Proof.
+  intros.
+  unfold context.
+  destruct ctx.
+  destruct p0.
+  destruct p0.
+  destruct p0.
+  eapply astar_DlyFrameFree; eauto.
+  eapply Context_DlyFrameFree'; eauto.
+Qed.
+
+Lemma Stack_DlyFrameFree' :
+  forall lfp l,
+    DlyFrameFree (stack' l lfp).
+Proof.
+  intro lfp.
+  induction lfp; intros.
+  -
+    simpls; eauto.
+  -
+    destruct a.
+    simpl.
+    repeat (split; eauto).
+    destruct f.
+    simpl.
+    repeat (split; eauto).
+    destruct f0.
+    simpl.
+    repeat (split; eauto).
+Qed.
+
+Lemma Stack_DlyFrameFree :
+  forall stk p,
+    DlyFrameFree p -> DlyFrameFree (stack stk ** p).
+Proof.
+  intros.
+  unfold stack.
+  destruct stk; eauto.
+  eapply astar_DlyFrameFree; eauto.
+  eapply Stack_DlyFrameFree'; eauto.
+Qed.
+  
+Ltac DlyFrameFree_elim :=
+  match goal with
+  | |- DlyFrameFree (Atrue ** ?p) =>
+    eapply Atrue_DlyFrameFree; DlyFrameFree_elim
+  | |- DlyFrameFree (Afalse ** ?p) =>
+    eapply Afalse_DlyFrameFree; DlyFrameFree_elim
+  | |- DlyFrameFree (?rn |=> ?v ** ?p) =>
+    eapply RegSt_DlyFrameFree; DlyFrameFree_elim
+  | |- DlyFrameFree (?l |-> ?v ** ?p) =>
+    eapply MapSto_DlyFrameFree; DlyFrameFree_elim
+  | |- DlyFrameFree (context ?ctx ** ?p) =>
+    eapply Context_DlyFrameFree; DlyFrameFree_elim
+  | |- DlyFrameFree (stack ?stk ** ?p) =>
+    eapply Stack_DlyFrameFree; DlyFrameFree_elim
+  | _ =>
+    try solve [simpl; eauto]
+  end.
