coqimp/contextswitch/proof/WindowOKProof.v
@@ -1,0 +1,185 @@
+Require Import Coqlib.                          
+Require Import Maps.           
+Require Import LibTactics.   
+        
+Require Import Integers.  
+Open Scope Z_scope.        
+Import ListNotations.  
+   
+Set Asymmetric Patterns.  
+        
+Require Import state.    
+Require Import language. 
+ 
+Set Implicit Arguments.    
+Unset Strict Implicit. 
+               
+Require Import logic.
+    
+Require Import lemmas.
+Require Import lemmas_ins.
+
+Require Import Coq.Logic.FunctionalExtensionality.
+
+Require Import integer_lemma.
+
+Require Import sep_lemma.
+Require Import reg_lemma.
+Require Import derived_rule.
+
+Require Import tm_dly_lemma.
+
+Require Import code.
+Require Import ctxswitch_spec.
+
+Require Import lemma1.
+
+Open Scope nat.
+Open Scope code_scope.
+Open Scope mem_scope.
+
+(*+ Lemmas for Integer +*)
+Lemma in_range84 :
+  ($ (-4096)) <=ᵢ ($ 84) && ($ 84) <=ᵢ ($ 4095) = true.
+Proof.
+  unfold orb.
+  unfold Int.lt.
+  unfold Int.eq.
+  destruct (zlt (Int.signed $ (-4096)) (Int.signed $ 84)) eqn:Heqe;
+    destruct (zeq (Int.unsigned $ (-4096)) (Int.unsigned $ 84)) eqn:Heqe1;
+    destruct (zlt (Int.signed $ 84) (Int.signed $ 4095)) eqn:Heqe2;
+    destruct (zeq (Int.unsigned $ 84) (Int.unsigned $ 4095)) eqn:Heqe3; eauto; tryfalse.
+Qed.
+
+Theorem Ta0WindowOKProof :
+  forall vl,
+    spec |- {{ ta0_window_ok_pre vl }}
+             ta0_window_ok
+           {{ ta0_window_ok_post vl }}.
+Proof.
+  intros.
+  unfold ta0_window_ok_pre.
+  unfold ta0_window_ok_post.
+  hoare_ex_intro_pre. 
+  renames x' to fmg, x'0 to fmo, x'1 to fml, x'2 to fmi, x'3 to id, x'4 to F.
+  renames x'5 to vy, x'6 to vi, x'7 to ll. 
+  renames x'8 to ct, x'9 to cctx, x'10 to cstk, x'11 to nt, x'12 to nctx, x'13 to nstk.
+  renames x'14 to vz, x'15 to vn. 
+  eapply Pure_intro_rule; introv Hlgvl.
+  hoare_lift_pre 13.
+  eapply Pure_intro_rule; introv Hpt_ctx.
+  hoare_lift_pre 13.
+  eapply Pure_intro_rule; introv Hneq_cwp_invalid.
+  hoare_lift_pre 15.
+  eapply Pure_intro_rule; introv Hct.
+  hoare_lift_pre 15.
+  eapply Pure_intro_rule; introv Hnt.
+  hoare_lift_pre 15.
+  eapply Pure_intro_rule; introv Hst_fm_constraint.
+  
+  unfold ta0_window_ok.
+  destruct fmg, fmo, fml, fmi.
+  hoare_lift_pre 2.
+
+  eapply backward_rule.
+  introv Hs.
+  eapply Regs_Global_combine_GenRegs in Hs; eauto.
+
+  (** set OSIntNestCnt l4 *)
+  eapply seq_rule.
+  TimReduce_simpl.
+  eapply set_rule_reg; eauto.
+  simpl upd_genreg.
+
+  (** ld [l4] l5 *)
+  hoare_lift_pre 9.
+  hoare_lift_pre 2.
+  eapply seq_rule.
+  TimReduce_simpl.
+  eapply ld_rule_reg; eauto.
+  simpl upd_genreg.
+
+  (** add l5 1 l5 *)
+  eapply seq_rule.
+  TimReduce_simpl.
+  eapply add_rule_reg; eauto.
+  simpl.
+  rewrite in_range1; eauto.
+  simpl upd_genreg.
+
+  (** st l5 [l4] *)
+  eapply seq_rule.
+  TimReduce_simpl.
+  eapply st_rule_reg; eauto.
+  simpl get_genreg_val.
+
+  (** set OSTaskCur l4 *)
+  eapply seq_rule.
+  TimReduce_simpl.
+  eapply set_rule_reg; eauto.
+  simpl upd_genreg.
+
+  (** ld [l4] l4 *)
+  hoare_lift_pre 7.
+  hoare_lift_pre 2.
+  eapply seq_rule.
+  TimReduce_simpl.
+  eapply ld_rule_reg; eauto.
+  simpl upd_genreg.
+
+  (** subcc l4 0 g0 *)
+  hoare_lift_pre 6.
+  hoare_lift_pre 7.
+  hoare_lift_pre 3.
+  eapply seq_rule.
+  TimReduce_simpl.
+  eapply subcc_rule_reg; eauto.
+  simpl.
+  rewrite in_range0; eauto.
+  simpl upd_genreg.
+  simpl get_genreg_val.
+
+  (** be Ta0_start_adjust_cwp; nop *)
+  eapply Be_rule.
+  {
+    (** spec waits to add *)
+    admit.
+  }
+  {
+    TimReduce_simpl.
+    eapply nop_rule; eauto.
+  }
+  {
+    TimReduce_simpl.
+    introv Hs.
+    simpl_sep_liftn_in Hs 3.
+    sep_cancel1 1 1.
+    simpl; eauto.
+  }
+
+  Focus 2.
+  admit.
+
+  Focus 2.
+  admit.
+
+  introv Hiszero.
+  unfold iszero in Hiszero.
+  eapply int_eq_true_eq in Hiszero.
+  destruct (Int.eq_dec ct -ᵢ ($ 0) $ 0); tryfalse.
+  renames n to Hct_no_null.
+  rewrite Int.sub_zero_l in Hct_no_null.
+  lets Hct_ctx_offset : Hct_no_null.
+  eapply Hct in Hct_ctx_offset.
+
+  (** add l4 OS_CONTEXT_OFFSET l5 *)
+  eapply seq_rule.
+  TimReduce_simpl.
+  eapply add_rule_reg; eauto.
+  simpl.
+  unfold OS_CONTEXT_OFFSET.
+  rewrite in_range84; eauto.
+  simpl upd_genreg.
+
+Admitted.
+  
