coqimp/contextswitch/proof/lemma1.v
@@ -1,0 +1,978 @@
+Require Import Coqlib.                         
+Require Import Maps.           
+Require Import LibTactics.   
+        
+Require Import Integers.  
+Open Scope Z_scope.        
+Import ListNotations.  
+   
+Set Asymmetric Patterns.  
+        
+Require Import state.    
+Require Import language. 
+ 
+Set Implicit Arguments.    
+Unset Strict Implicit. 
+               
+Require Import logic.
+    
+Require Import lemmas.
+Require Import lemmas_ins.
+
+Require Import Coq.Logic.FunctionalExtensionality.
+
+Require Import sep_lemma.
+Require Import reg_lemma.
+Require Import derived_rule.
+
+Require Import integer_lemma.
+
+Require Import code.
+Require Import ctxswitch_spec.
+
+Open Scope nat.
+Open Scope code_scope.
+Open Scope mem_scope.
+
+(*+ Trivial Lemmas +*)
+Lemma len_neq_0_tail :
+  forall {A : Type} (ls : list A),
+    length ls > 0 -> exists a ls', ls = ls' ++ (a :: nil).
+Proof.
+  intros A ls.
+  induction ls; intros.
+  -
+    simpls; tryfalse.
+    omega.
+  -
+    destruct ls.
+    exists a.
+    eexists.
+    instantiate (1 := nil).
+    simpl; eauto.
+    assert (length (a0 :: ls) > 0).
+    simpl; eauto.
+    omega.
+    eapply IHls in H0.
+    simpljoin1.
+    exists x (a :: x0).
+    simpl; eauto.
+    rewrite H0.
+    eauto.
+Qed.
+
+(*+ Lemmas for asrt +*)
+Lemma asrt_disj_intro :
+  forall p1 p2 s,
+    s |= p1 \/ s |= p2 ->
+    s |= p1 \\// p2.
+Proof.
+  intros.
+  simpl.
+  eauto.
+Qed.
+
+(*+ Lemmas for Rules +*)
+Lemma rd_rule_reg_wim :
+  forall (v id : Word) (rr : GenReg) (p : asrt) F (grst : GenRegState),
+    |- {{GenRegs grst ** FrameState id v F ** p}} rd Rwim rr
+      {{GenRegs (upd_genreg grst rr (($ 1) <<ᵢ v)) ** FrameState id v F ** p}}.
+Proof.
+  intros.
+  eapply ins_conseq_rule.
+  introv Hs. 
+  simpl_sep_liftn_in Hs 2.
+  unfold FrameState in Hs.
+  eapply astar_assoc_elim in Hs.
+  simpl_sep_liftn_in Hs 2.
+  eapply astar_assoc_elim in Hs.
+  simpl_sep_liftn_in Hs 4.
+  eauto.
+  eapply rd_rule_reg.
+  introv Hs.
+  sep_cancel1 1 1.
+  unfold FrameState.
+  eapply astar_assoc_intro.
+  sep_cancel1 3 1.
+  eapply astar_assoc_intro.
+  sep_cancel1 1 1.
+  eauto.
+Qed.
+
+Theorem save_rule_reg_frame :
+  forall p (rs rd : GenReg) (id id' : Word) (F : FrameList)
+    (fm1 fm2 fmg fmo fml fmi : Frame) (v1 v2 v v' : Word) (oexp : OpExp),
+    get_genreg_val (fmg, fmo, fml, fmi) rs = v1 ->
+    eval_opexp_reg (fmg, fmo, fml, fmi) oexp = Some v2 ->
+    id' = pre_cwp id -> win_masked id' (($ 1) <<ᵢ v) = false ->
+    |- {{ GenRegs (fmg, fmo, fml, fmi) ** FrameState id v (F ++ fm1 :: fm2 :: nil) ** p }}
+        save rs oexp rd
+        {{ GenRegs (upd_genreg (fmg, fm1, fm2, fmo) rd (v1 +ᵢ v2)) **
+                   FrameState id' v (fml :: fmi :: F) ** p }}.
+Proof.
+  intros.
+  eapply ins_conseq_rule.
+  Focus 2.
+  eapply save_rule_reg; eauto.
+  {
+    introv Hs.
+    instantiate (4 := F).
+    instantiate (3 := fm1).
+    instantiate (2 := fm2).
+    instantiate (1 := [|length (fml :: fmi :: F) = 13|]
+                        ** [|$ 0 <=ᵤᵢ id' <=ᵤᵢ $ 7 /\ $ 0 <=ᵤᵢ v <=ᵤᵢ $ 7|] ** p).
+    unfolds FrameState.
+    sep_cancel1 1 1.
+    eapply astar_assoc_elim in H3.
+    sep_cancel1 1 2.
+    eapply astar_assoc_elim in H4.
+    sep_cancel1 1 1.
+    eapply astar_assoc_elim in H3.
+    eapply sep_pure_l_elim in H3.
+    simpljoin1.
+    eapply sep_pure_l_elim in H4.
+    simpljoin1; eauto.
+    eapply sep_pure_l_intro.
+    rewrite app_length in H3.
+    simpls.
+    omega. 
+    eapply sep_pure_l_intro; eauto.
+    split; eauto.
+    eapply in_range_0_7_pre_cwp_still; eauto.
+  }
+  {
+    introv Hs.
+    sep_cancel1 1 1.
+    unfold FrameState.
+    eapply astar_assoc_intro.
+    sep_cancel1 2 1.
+    eapply astar_assoc_intro.
+    sep_cancel1 1 1.
+    eapply astar_assoc_intro; eauto.
+  }
+Qed.
+
+Lemma st_rule_save_stk_l0 :
+  forall grst p l fm1 fm2 v1,
+    get_genreg_val grst l0 = v1 ->
+    get_genreg_val grst sp = l ->
+    |- {{ GenRegs grst ** stack_frame l fm1 fm2 ** p }}
+        st l0 (Aro sp (' 0))
+      {{ GenRegs grst ** stack_frame l (update_frame fm1 0 v1) fm2 ** p }}.
+Proof.
+  intros.
+  destruct fm1, fm2.
+  eapply ins_conseq_rule.
+  {
+    introv Hs.
+    simpl_sep_liftn_in Hs 2.
+    unfold stack_frame in Hs.
+    eapply astar_assoc_elim in Hs.
+    unfold stack_seg at 1 in Hs.
+    asrt_to_line_in Hs 7.
+    simpl_sep_liftn_in Hs 10.    
+    eauto.
+  }
+  { 
+    eapply st_rule_reg.
+    simpl.
+    rewrite in_range0; eauto.
+    rewrite H0; eauto.
+    rewrite Int.add_zero; eauto.
+    eauto.
+  }
+  {  
+    introv Hs.
+    simpl update_frame.
+    unfold stack_frame.
+    sep_cancel1 1 1.
+    eapply astar_assoc_intro.
+    sep_cancel1 9 2.
+    unfold stack_seg.
+    asrt_to_line 7. 
+    sep_cancel1 1 1.
+    eauto.
+  }
+Qed.
+
+Lemma st_rule_save_stk_l1 :
+  forall grst p l fm1 fm2 v1,
+    get_genreg_val grst l1 = v1 ->
+    get_genreg_val grst sp = l ->
+    |- {{ GenRegs grst ** stack_frame l fm1 fm2 ** p }}
+        st l1 (Aro sp (' 4))
+      {{ GenRegs grst ** stack_frame l (update_frame fm1 1 v1) fm2 ** p }}.
+Proof.
+  intros.
+  destruct fm1, fm2.
+  eapply ins_conseq_rule.
+  {
+    introv Hs.
+    simpl_sep_liftn_in Hs 2.
+    unfold stack_frame in Hs.
+    eapply astar_assoc_elim in Hs.
+    unfold stack_seg at 1 in Hs.
+    asrt_to_line_in Hs 7.
+    simpl_sep_liftn_in Hs 2.
+    simpl_sep_liftn_in Hs 10.    
+    eauto.
+  }
+  { 
+    eapply st_rule_reg.
+    simpl.
+    rewrite in_range4; eauto.
+    rewrite H0; eauto.
+    eauto.
+  }
+  {  
+    introv Hs.
+    simpl update_frame.
+    unfold stack_frame.
+    sep_cancel1 1 1.
+    eapply astar_assoc_intro.
+    sep_cancel1 9 2.
+    unfold stack_seg.
+    asrt_to_line 7.
+    sep_cancel1 1 2.
+    eauto.
+  }
+Qed.
+
+Lemma st_rule_save_stk_l2 :
+  forall grst p l fm1 fm2 v1,
+    get_genreg_val grst l2 = v1 ->
+    get_genreg_val grst sp = l ->
+    |- {{ GenRegs grst ** stack_frame l fm1 fm2 ** p }}
+        st l2 (Aro sp (' 8))
+      {{ GenRegs grst ** stack_frame l (update_frame fm1 2 v1) fm2 ** p }}.
+Proof.
+  intros.
+  destruct fm1, fm2.
+  eapply ins_conseq_rule.
+  {
+    introv Hs.
+    simpl_sep_liftn_in Hs 2.
+    unfold stack_frame in Hs.
+    eapply astar_assoc_elim in Hs.
+    unfold stack_seg at 1 in Hs.
+    asrt_to_line_in Hs 7.
+    simpl_sep_liftn_in Hs 3.
+    simpl_sep_liftn_in Hs 10.    
+    eauto.
+  }
+  { 
+    eapply st_rule_reg.
+    simpl.
+    rewrite in_range8; eauto.
+    rewrite H0; eauto.
+    eauto.
+  }
+  {  
+    introv Hs.
+    simpl update_frame.
+    unfold stack_frame.
+    sep_cancel1 1 1.
+    eapply astar_assoc_intro.
+    sep_cancel1 9 2.
+    unfold stack_seg.
+    asrt_to_line 7.
+    sep_cancel1 1 3.
+    eauto.
+  }
+Qed.
+
+Lemma st_rule_save_stk_l3 :
+  forall grst p l fm1 fm2 v1,
+    get_genreg_val grst l3 = v1 ->
+    get_genreg_val grst sp = l ->
+    |- {{ GenRegs grst ** stack_frame l fm1 fm2 ** p }}
+        st l3 (Aro sp (' 12))
+      {{ GenRegs grst ** stack_frame l (update_frame fm1 3 v1) fm2 ** p }}.
+Proof.
+  intros.
+  destruct fm1, fm2.
+  eapply ins_conseq_rule.
+  {
+    introv Hs.
+    simpl_sep_liftn_in Hs 2.
+    unfold stack_frame in Hs.
+    eapply astar_assoc_elim in Hs.
+    unfold stack_seg at 1 in Hs.
+    asrt_to_line_in Hs 7.
+    simpl_sep_liftn_in Hs 4.
+    simpl_sep_liftn_in Hs 10.    
+    eauto.
+  }
+  { 
+    eapply st_rule_reg.
+    simpl.
+    rewrite in_range12; eauto.
+    rewrite H0; eauto.
+    eauto.
+  }
+  {  
+    introv Hs.
+    simpl update_frame.
+    unfold stack_frame.
+    sep_cancel1 1 1.
+    eapply astar_assoc_intro.
+    sep_cancel1 9 2.
+    unfold stack_seg.
+    asrt_to_line 7.
+    sep_cancel1 1 4.
+    eauto.
+  }
+Qed.
+
+Lemma st_rule_save_stk_l4 :
+  forall grst p l fm1 fm2 v1,
+    get_genreg_val grst l4 = v1 ->
+    get_genreg_val grst sp = l ->
+    |- {{ GenRegs grst ** stack_frame l fm1 fm2 ** p }}
+        st l4 (Aro sp (' 16))
+      {{ GenRegs grst ** stack_frame l (update_frame fm1 4 v1) fm2 ** p }}.
+Proof.
+  intros.
+  destruct fm1, fm2.
+  eapply ins_conseq_rule.
+  {
+    introv Hs.
+    simpl_sep_liftn_in Hs 2.
+    unfold stack_frame in Hs.
+    eapply astar_assoc_elim in Hs.
+    unfold stack_seg at 1 in Hs.
+    asrt_to_line_in Hs 7.
+    simpl_sep_liftn_in Hs 5.
+    simpl_sep_liftn_in Hs 10.    
+    eauto.
+  }
+  { 
+    eapply st_rule_reg.
+    simpl.
+    rewrite in_range16; eauto.
+    rewrite H0; eauto.
+    eauto.
+  }
+  {  
+    introv Hs.
+    simpl update_frame.
+    unfold stack_frame.
+    sep_cancel1 1 1.
+    eapply astar_assoc_intro.
+    sep_cancel1 9 2.
+    unfold stack_seg.
+    asrt_to_line 7.
+    sep_cancel1 1 5.
+    eauto.
+  }
+Qed.
+
+Lemma st_rule_save_stk_l5 :
+  forall grst p l fm1 fm2 v1,
+    get_genreg_val grst l5 = v1 ->
+    get_genreg_val grst sp = l ->
+    |- {{ GenRegs grst ** stack_frame l fm1 fm2 ** p }}
+        st l5 (Aro sp (' 20))
+      {{ GenRegs grst ** stack_frame l (update_frame fm1 5 v1) fm2 ** p }}.
+Proof.
+  intros.
+  destruct fm1, fm2.
+  eapply ins_conseq_rule.
+  {
+    introv Hs.
+    simpl_sep_liftn_in Hs 2.
+    unfold stack_frame in Hs.
+    eapply astar_assoc_elim in Hs.
+    unfold stack_seg at 1 in Hs.
+    asrt_to_line_in Hs 7.
+    simpl_sep_liftn_in Hs 6.
+    simpl_sep_liftn_in Hs 10.    
+    eauto.
+  }
+  { 
+    eapply st_rule_reg.
+    simpl.
+    rewrite in_range20; eauto.
+    rewrite H0; eauto.
+    eauto.
+  }
+  {  
+    introv Hs.
+    simpl update_frame.
+    unfold stack_frame.
+    sep_cancel1 1 1.
+    eapply astar_assoc_intro.
+    sep_cancel1 9 2.
+    unfold stack_seg.
+    asrt_to_line 7.
+    sep_cancel1 1 6.
+    eauto.
+  }
+Qed.
+
+Lemma st_rule_save_stk_l6 :
+  forall grst p l fm1 fm2 v1,
+    get_genreg_val grst l6 = v1 ->
+    get_genreg_val grst sp = l ->
+    |- {{ GenRegs grst ** stack_frame l fm1 fm2 ** p }}
+        st l6 (Aro sp (' 24))
+      {{ GenRegs grst ** stack_frame l (update_frame fm1 6 v1) fm2 ** p }}.
+Proof.
+  intros.
+  destruct fm1, fm2.
+  eapply ins_conseq_rule.
+  {
+    introv Hs.
+    simpl_sep_liftn_in Hs 2.
+    unfold stack_frame in Hs.
+    eapply astar_assoc_elim in Hs.
+    unfold stack_seg at 1 in Hs.
+    asrt_to_line_in Hs 7.
+    simpl_sep_liftn_in Hs 7.
+    simpl_sep_liftn_in Hs 10.    
+    eauto.
+  }
+  { 
+    eapply st_rule_reg.
+    simpl.
+    rewrite in_range24; eauto.
+    rewrite H0; eauto.
+    eauto.
+  }
+  {  
+    introv Hs.
+    simpl update_frame.
+    unfold stack_frame.
+    sep_cancel1 1 1.
+    eapply astar_assoc_intro.
+    sep_cancel1 9 2.
+    unfold stack_seg.
+    asrt_to_line 7.
+    sep_cancel1 1 7.
+    eauto.
+  }
+Qed.
+
+Lemma st_rule_save_stk_l7 :
+  forall grst p l fm1 fm2 v1,
+    get_genreg_val grst l7 = v1 ->
+    get_genreg_val grst sp = l ->
+    |- {{ GenRegs grst ** stack_frame l fm1 fm2 ** p }}
+        st l7 (Aro sp (' 28))
+      {{ GenRegs grst ** stack_frame l (update_frame fm1 7 v1) fm2 ** p }}.
+Proof.
+  intros.
+  destruct fm1, fm2.
+  eapply ins_conseq_rule.
+  {
+    introv Hs.
+    simpl_sep_liftn_in Hs 2.
+    unfold stack_frame in Hs.
+    eapply astar_assoc_elim in Hs.
+    unfold stack_seg at 1 in Hs.
+    asrt_to_line_in Hs 7.
+    simpl_sep_liftn_in Hs 8.
+    simpl_sep_liftn_in Hs 10.    
+    eauto.
+  }
+  { 
+    eapply st_rule_reg.
+    simpl.
+    rewrite in_range28; eauto.
+    rewrite H0; eauto.
+    eauto.
+  }
+  {  
+    introv Hs.
+    simpl update_frame.
+    unfold stack_frame.
+    sep_cancel1 1 1.
+    eapply astar_assoc_intro.
+    sep_cancel1 9 2.
+    unfold stack_seg.
+    asrt_to_line 7.
+    sep_cancel1 1 8.
+    eauto.
+  }
+Qed.
+
+Lemma st_rule_save_stk_i0 :
+  forall grst p l fm1 fm2 v1, 
+    get_genreg_val grst i0 = v1 ->
+    get_genreg_val grst sp = l ->
+    |- {{ GenRegs grst ** stack_frame l fm1 fm2 ** p }}
+        st i0 (Aro sp (' 32))
+      {{ GenRegs grst ** stack_frame l fm1 (update_frame fm2 0 v1) ** p }}.
+Proof.
+  intros.
+  destruct fm1, fm2.
+  eapply ins_conseq_rule.
+  {
+    introv Hs.
+    simpl_sep_liftn_in Hs 2.
+    unfold stack_frame in Hs.
+    eapply astar_assoc_elim in Hs.
+    simpl_sep_liftn_in Hs 2.
+    unfold stack_seg at 1 in Hs.
+    asrt_to_line_in Hs 7.
+    simpl_sep_liftn_in Hs 10.    
+    eauto.
+  }
+  { 
+    eapply st_rule_reg.
+    simpl.
+    rewrite in_range32; eauto.
+    rewrite H0; eauto.
+    eauto.
+  }
+  {  
+    introv Hs.
+    simpl update_frame.
+    unfold stack_frame.
+    sep_cancel1 1 1.
+    eapply astar_assoc_intro.
+    sep_cancel1 9 1.
+    unfold stack_seg.
+    asrt_to_line 7.
+    eauto.
+  }
+Qed.
+
+Lemma st_rule_save_stk_i1 :
+  forall grst p l fm1 fm2 v1,
+    get_genreg_val grst i1 = v1 ->
+    get_genreg_val grst sp = l ->
+    |- {{ GenRegs grst ** stack_frame l fm1 fm2 ** p }}
+        st i1 (Aro sp (' 36))
+      {{ GenRegs grst ** stack_frame l fm1 (update_frame fm2 1 v1) ** p }}.
+Proof.
+  intros.
+  destruct fm1, fm2.
+  eapply ins_conseq_rule.
+  {
+    introv Hs.
+    simpl_sep_liftn_in Hs 2.
+    unfold stack_frame in Hs.
+    eapply astar_assoc_elim in Hs.
+    simpl_sep_liftn_in Hs 2.
+    unfold stack_seg at 1 in Hs.
+    asrt_to_line_in Hs 7.
+    simpl_sep_liftn_in Hs 2.
+    simpl_sep_liftn_in Hs 10.    
+    eauto.
+  }
+  { 
+    eapply st_rule_reg.
+    simpl.
+    rewrite in_range36; eauto.
+    rewrite H0; eauto.
+    rewrite Int.add_assoc.
+    eauto.
+    eauto.
+  }
+  {  
+    introv Hs.
+    simpl update_frame.
+    unfold stack_frame.
+    sep_cancel1 1 1.
+    eapply astar_assoc_intro.
+    sep_cancel1 9 1.
+    unfold stack_seg.
+    asrt_to_line 7. 
+    sep_cancel1 1 2.
+    eauto.
+  }
+Qed.
+
+Lemma st_rule_save_stk_i2 :
+  forall grst p l fm1 fm2 v1,
+    get_genreg_val grst i2 = v1 ->
+    get_genreg_val grst sp = l ->
+    |- {{ GenRegs grst ** stack_frame l fm1 fm2 ** p }}
+        st i2 (Aro sp (' 40))
+      {{ GenRegs grst ** stack_frame l fm1 (update_frame fm2 2 v1) ** p }}.
+Proof.
+  intros.
+  destruct fm1, fm2.
+  eapply ins_conseq_rule.
+  {
+    introv Hs.
+    simpl_sep_liftn_in Hs 2.
+    unfold stack_frame in Hs.
+    eapply astar_assoc_elim in Hs.
+    simpl_sep_liftn_in Hs 2.
+    unfold stack_seg at 1 in Hs.
+    asrt_to_line_in Hs 7.
+    simpl_sep_liftn_in Hs 3.
+    simpl_sep_liftn_in Hs 10.    
+    eauto.
+  }
+  { 
+    eapply st_rule_reg.
+    simpl.
+    rewrite in_range40; eauto.
+    rewrite H0; eauto.
+    rewrite Int.add_assoc.
+    eauto.
+    eauto.
+  }
+  {  
+    introv Hs.
+    simpl update_frame.
+    unfold stack_frame.
+    sep_cancel1 1 1.
+    eapply astar_assoc_intro.
+    sep_cancel1 9 1.
+    unfold stack_seg.
+    asrt_to_line 7. 
+    sep_cancel1 1 3. 
+    eauto.
+  }
+Qed.
+
+Lemma st_rule_save_stk_i3 :
+  forall grst p l fm1 fm2 v1,
+    get_genreg_val grst i3 = v1 ->
+    get_genreg_val grst sp = l ->
+    |- {{ GenRegs grst ** stack_frame l fm1 fm2 ** p }}
+        st i3 (Aro sp (' 44))
+      {{ GenRegs grst ** stack_frame l fm1 (update_frame fm2 3 v1) ** p }}.
+Proof.
+  intros.
+  destruct fm1, fm2.
+  eapply ins_conseq_rule.
+  {
+    introv Hs.
+    simpl_sep_liftn_in Hs 2.
+    unfold stack_frame in Hs.
+    eapply astar_assoc_elim in Hs.
+    simpl_sep_liftn_in Hs 2.
+    unfold stack_seg at 1 in Hs.
+    asrt_to_line_in Hs 7.
+    simpl_sep_liftn_in Hs 4.
+    simpl_sep_liftn_in Hs 10.    
+    eauto.
+  }
+  { 
+    eapply st_rule_reg.
+    simpl.
+    rewrite in_range44; eauto.
+    rewrite H0; eauto.
+    rewrite Int.add_assoc.
+    eauto.
+    eauto.
+  }
+  {  
+    introv Hs.
+    simpl update_frame.
+    unfold stack_frame.
+    sep_cancel1 1 1.
+    eapply astar_assoc_intro.
+    sep_cancel1 9 1.
+    unfold stack_seg.
+    asrt_to_line 7. 
+    sep_cancel1 1 4. 
+    eauto.
+  }
+Qed.
+
+Lemma st_rule_save_stk_i4 :
+  forall grst p l fm1 fm2 v1,
+    get_genreg_val grst i4 = v1 ->
+    get_genreg_val grst sp = l ->
+    |- {{ GenRegs grst ** stack_frame l fm1 fm2 ** p }}
+        st i4 (Aro sp (' 48))
+      {{ GenRegs grst ** stack_frame l fm1 (update_frame fm2 4 v1) ** p }}.
+Proof.
+  intros.
+  destruct fm1, fm2.
+  eapply ins_conseq_rule.
+  {
+    introv Hs.
+    simpl_sep_liftn_in Hs 2.
+    unfold stack_frame in Hs.
+    eapply astar_assoc_elim in Hs.
+    simpl_sep_liftn_in Hs 2.
+    unfold stack_seg at 1 in Hs.
+    asrt_to_line_in Hs 7.
+    simpl_sep_liftn_in Hs 5.
+    simpl_sep_liftn_in Hs 10.    
+    eauto.
+  }
+  { 
+    eapply st_rule_reg.
+    simpl. 
+    rewrite in_range48; eauto.
+    rewrite H0; eauto.
+    rewrite Int.add_assoc.
+    eauto.
+    eauto.
+  }
+  {  
+    introv Hs.
+    simpl update_frame.
+    unfold stack_frame.
+    sep_cancel1 1 1.
+    eapply astar_assoc_intro.
+    sep_cancel1 9 1.
+    unfold stack_seg.
+    asrt_to_line 7. 
+    sep_cancel1 1 5. 
+    eauto.
+  }
+Qed.
+
+Lemma st_rule_save_stk_i5 :
+  forall grst p l fm1 fm2 v1,
+    get_genreg_val grst i5 = v1 ->
+    get_genreg_val grst sp = l ->
+    |- {{ GenRegs grst ** stack_frame l fm1 fm2 ** p }}
+        st i5 (Aro sp (' 52))
+      {{ GenRegs grst ** stack_frame l fm1 (update_frame fm2 5 v1) ** p }}.
+Proof.
+  intros.
+  destruct fm1, fm2.
+  eapply ins_conseq_rule.
+  {
+    introv Hs.
+    simpl_sep_liftn_in Hs 2.
+    unfold stack_frame in Hs.
+    eapply astar_assoc_elim in Hs.
+    simpl_sep_liftn_in Hs 2.
+    unfold stack_seg at 1 in Hs.
+    asrt_to_line_in Hs 7.
+    simpl_sep_liftn_in Hs 6.
+    simpl_sep_liftn_in Hs 10.    
+    eauto.
+  }
+  { 
+    eapply st_rule_reg.
+    simpl. 
+    rewrite in_range52; eauto.
+    rewrite H0; eauto.
+    rewrite Int.add_assoc.
+    eauto.
+    eauto.
+  }
+  {  
+    introv Hs.
+    simpl update_frame.
+    unfold stack_frame.
+    sep_cancel1 1 1.
+    eapply astar_assoc_intro.
+    sep_cancel1 9 1.
+    unfold stack_seg.
+    asrt_to_line 7. 
+    sep_cancel1 1 6. 
+    eauto.
+  }
+Qed.
+
+Lemma st_rule_save_stk_i6 :
+  forall grst p l fm1 fm2 v1,
+    get_genreg_val grst i6 = v1 ->
+    get_genreg_val grst sp = l ->
+    |- {{ GenRegs grst ** stack_frame l fm1 fm2 ** p }}
+        st i6 (Aro sp (' 56))
+      {{ GenRegs grst ** stack_frame l fm1 (update_frame fm2 6 v1) ** p }}.
+Proof.
+  intros.
+  destruct fm1, fm2.
+  eapply ins_conseq_rule.
+  {
+    introv Hs.
+    simpl_sep_liftn_in Hs 2.
+    unfold stack_frame in Hs.
+    eapply astar_assoc_elim in Hs.
+    simpl_sep_liftn_in Hs 2.
+    unfold stack_seg at 1 in Hs.
+    asrt_to_line_in Hs 7.
+    simpl_sep_liftn_in Hs 7.
+    simpl_sep_liftn_in Hs 10.    
+    eauto.
+  }
+  { 
+    eapply st_rule_reg.
+    simpl. 
+    rewrite in_range56; eauto.
+    rewrite H0; eauto.
+    rewrite Int.add_assoc.
+    eauto.
+    eauto.
+  }
+  {  
+    introv Hs.
+    simpl update_frame.
+    unfold stack_frame.
+    sep_cancel1 1 1.
+    eapply astar_assoc_intro.
+    sep_cancel1 9 1.
+    unfold stack_seg.
+    asrt_to_line 7. 
+    sep_cancel1 1 7. 
+    eauto.
+  }
+Qed.
+
+Lemma st_rule_save_stk_i7 :
+  forall grst p l fm1 fm2 v1,
+    get_genreg_val grst i7 = v1 ->
+    get_genreg_val grst sp = l ->
+    |- {{ GenRegs grst ** stack_frame l fm1 fm2 ** p }}
+        st i7 (Aro sp (' 60))
+      {{ GenRegs grst ** stack_frame l fm1 (update_frame fm2 7 v1) ** p }}.
+Proof.
+  intros.
+  destruct fm1, fm2.
+  eapply ins_conseq_rule.
+  {
+    introv Hs.
+    simpl_sep_liftn_in Hs 2.
+    unfold stack_frame in Hs.
+    eapply astar_assoc_elim in Hs.
+    simpl_sep_liftn_in Hs 2.
+    unfold stack_seg at 1 in Hs.
+    asrt_to_line_in Hs 7.
+    simpl_sep_liftn_in Hs 8.
+    simpl_sep_liftn_in Hs 10.    
+    eauto.
+  }
+  { 
+    eapply st_rule_reg.
+    simpl. 
+    rewrite in_range60; eauto.
+    rewrite H0; eauto.
+    rewrite Int.add_assoc.
+    eauto.
+    eauto.
+  }
+  {  
+    introv Hs.
+    simpl update_frame.
+    unfold stack_frame.
+    sep_cancel1 1 1.
+    eapply astar_assoc_intro.
+    sep_cancel1 9 1.
+    unfold stack_seg.
+    asrt_to_line 7. 
+    sep_cancel1 1 8. 
+    eauto.
+  }
+Qed.
+  
+(*+ Lemmas for stack frame constraint +*)
+Lemma stack_frame_constraint_pt_same_equal :
+  forall fm1 fm2 fm1' fm2' F id vi stk,
+    get_frame_nth fm2 6 = get_frame_nth fm2' 6 ->
+    stack_frame_constraint stk (fm1 :: fm2 :: F) id vi ->
+    stack_frame_constraint stk (fm1' :: fm2' :: F) id vi.
+Proof.
+  intros.
+  unfolds stack_frame_constraint.
+  inversion H0; subst.
+  {
+    eapply frame_invalid; eauto.
+  }
+  {
+    eapply frame_valid; eauto.
+    rewrite <- H; eauto.
+  }
+Qed.
+
+Lemma stk_bottom_pre_pt :
+  forall l id F fm1 fm2 fm3 l' lfp s p,
+    length F = 13 -> $ 0 <=ᵤᵢ id <=ᵤᵢ $ 7 ->
+    stack_frame_constraint' l id (F ++ fm1 :: fm2 :: fm3 :: nil) lfp id ->
+    get_frame_nth fm1 6 = Some l' -> s |= stack' l lfp ** p ->
+    s |= EX lfp1 lfp2 fm' fm'', stack' l lfp1 ** stack_frame l' fm' fm''
+         ** stack' (l' -ᵢ ($ 64)) lfp2 ** [| length lfp1 = 6 /\ l' = l -ᵢ ($ (64 * 6)) |] ** p.
+Proof.  
+  intros.
+  do 14 (try destruct F; simpl in H; tryfalse).
+  simpl in H1.
+  inversion H1; subst.
+  {
+    eapply post_1_neq in H4; eauto.
+    tryfalse.
+  }
+
+  inversion H13; subst.
+  {
+    eapply post_2_neq in H4; tryfalse; eauto.
+  }
+
+  clear H1 H9 H13 H10.
+  inversion H16; subst.
+  {
+    eapply post_3_neq in H1; eauto; tryfalse.
+  }
+
+  clear H12 H15 H16 H8 H11.
+  inversion H13; subst.
+  {
+    eapply post_4_neq in H1; eauto; tryfalse.
+  }
+
+  clear H13 H8 H11.
+  inversion H12; subst.
+  {
+    eapply post_5_neq in H1; eauto; tryfalse.
+  }
+
+  clear H12 H8 H11.
+  inversion H13; subst.
+  {
+    eapply post_6_neq in H1; eauto; tryfalse.
+  }
+
+  clear H13 H8 H11.
+  inversion H12; subst.
+  {
+    eapply post_7_eq in H1; eauto; tryfalse.
+  }
+  
+  clear H12 H8.
+  inversion H13; subst. 
+  sep_ex_intro.
+  instantiate
+    (5 := (fml', fmi')
+             :: (fml'0, fmi'0)
+                :: (fml'1, fmi'1)
+                :: (fml'2, fmi'2) :: (fml'3, fmi'3) :: (fml'4, fmi'4) :: nil).
+  instantiate (3 := fml'5).
+  instantiate (2 := fmi'5).
+  instantiate (1 := lfp0).  
+  clear - H3 H11 H2.
+  unfolds stack'. folds stack'.
+  do 6 (
+       match goal with
+       | H :  _ |= _ |- _ =>
+         eapply astar_assoc_elim in H
+       end;
+       eapply astar_assoc_intro; sep_cancel1 1 1).
+  rewrite H2 in H11.
+  inversion H11; subst.
+  eapply astar_assoc_elim in H0.
+  sep_cancel1 1 2.
+  sep_cancel1 1 2.
+  simpl_sep_liftn 2.
+  eapply sep_pure_l_intro; eauto.
+  split; simpl; eauto.
+  repeat (rewrite Int.sub_add_opp; eauto).
+  repeat (rewrite Int.add_assoc; eauto).
+  eapply astar_emp_intro_l; eauto.
+  eapply post_8_eq in H0.
+  eapply H8 in H0.
+  tryfalse.
+Qed.
+
+(*+ Lemmas for Space +*)
+Lemma stack_frame_combine :
+  forall l fm1 fm2 lfp s p,
+    s |= stack_frame l fm1 fm2 ** stack' (l -ᵢ ($ 64)) lfp ** p ->
+    s |= stack' l ((fm1, fm2) :: lfp) ** p.
+Proof.
+  intros.
+  unfold stack'; fold stack'.
+  eapply astar_assoc_intro; eauto.
+Qed.
